autoclrs/ch13-rbtree/CLRS.Ch13.RBTree.CLRSRubric.fst
@@ -38,6 +38,8 @@ let rec node_count (a:Type0) (t:rbtree a) : nat =
   | Leaf -> 0
   | Node _ l _ r -> 1 + node_count a l + node_count a r
 
+let empty_model (a:Type0) : GTot (rbtree a) = Leaf
+
 let rec find_model (a:Type0) (ord:erased (TO.total_order a)) (t:rbtree a) (key:a)
   : GTot (option a)
   =
@@ -48,6 +50,32 @@ let rec find_model (a:Type0) (ord:erased (TO.total_order a)) (t:rbtree a) (key:a
       if lt cmp then find_model a ord l key
       else if gt cmp then find_model a ord r key
       else Some k
+
+// ---- BST Predicates ----
+
+let lt_ord (a:Type0) (ord:erased (TO.total_order a)) (x y:a) : GTot bool =
+  lt (ord.TO.compare x y)
+
+let gt_ord (a:Type0) (ord:erased (TO.total_order a)) (x y:a) : GTot bool =
+  gt (ord.TO.compare x y)
+
+let rec all_lt (a:Type0) (ord:erased (TO.total_order a)) (t:rbtree a) (bound:a) : GTot bool =
+  match t with
+  | Leaf -> true
+  | Node _ l v r -> lt_ord a ord v bound && all_lt a ord l bound && all_lt a ord r bound
+
+let rec all_gt (a:Type0) (ord:erased (TO.total_order a)) (t:rbtree a) (bound:a) : GTot bool =
+  match t with
+  | Leaf -> true
+  | Node _ l v r -> gt_ord a ord v bound && all_gt a ord l bound && all_gt a ord r bound
+
+let rec is_bst (a:Type0) (ord:erased (TO.total_order a)) (t:rbtree a) : GTot bool =
+  match t with
+  | Leaf -> true
+  | Node _ l v r -> all_lt a ord l v && all_gt a ord r v && is_bst a ord l && is_bst a ord r
+
+let valid (a:Type0) (ord:erased (TO.total_order a)) (t:rbtree a) : GTot prop =
+  is_bst a ord t = true
 
 let is_red_node (a:Type0) (t:rbtree a) : bool =
   match t with
@@ -62,6 +90,146 @@ let set_color (a:Type0) (c:color) (t:rbtree a) : rbtree a =
 let make_black (a:Type0) (t:rbtree a) : rbtree a =
   set_color a Black t
 
+// ---- set_color is invariant for is_bst/all_lt/all_gt/find_model ----
+
+let set_color_is_bst (a:Type0) (ord:erased (TO.total_order a)) (c:color) (t:rbtree a)
+  : Lemma (ensures is_bst a ord (set_color a c t) == is_bst a ord t)
+  = match t with
+    | Leaf -> ()
+    | Node _ l k r -> ()
+
+let set_color_all_lt (a:Type0) (ord:erased (TO.total_order a)) (c:color) (t:rbtree a) (bound:a)
+  : Lemma (ensures all_lt a ord (set_color a c t) bound == all_lt a ord t bound)
+  = match t with
+    | Leaf -> ()
+    | Node _ l k r -> ()
+
+let set_color_all_gt (a:Type0) (ord:erased (TO.total_order a)) (c:color) (t:rbtree a) (bound:a)
+  : Lemma (ensures all_gt a ord (set_color a c t) bound == all_gt a ord t bound)
+  = match t with
+    | Leaf -> ()
+    | Node _ l k r -> ()
+
+let set_color_find (a:Type0) (ord:erased (TO.total_order a)) (c:color) (t:rbtree a) (key:a)
+  : Lemma (ensures find_model a ord (set_color a c t) key == find_model a ord t key)
+  = match t with
+    | Leaf -> ()
+    | Node _ l k r -> ()
+
+// ===== BST Weaken Lemmas =====
+
+let reveal_ord (a:Type0) (ord:erased (TO.total_order a)) : Lemma (
+  (forall (x y z:a). {:pattern ord.TO.compare x y; ord.TO.compare y z}
+    lt (ord.TO.compare x y) /\ lt (ord.TO.compare y z) ==> lt (ord.TO.compare x z)) /\
+  (forall (x y:a). {:pattern ord.TO.compare x y}
+    ord.TO.compare x y == TO.flip_order (ord.TO.compare y x)))
+  = let _ = ord.TO.properties in ()
+
+let compare_eq_is_eq (a:Type0) (ord:erased (TO.total_order a)) (x y:a)
+  : Lemma (requires eq (x `ord.TO.compare` y)) (ensures x == y)
+  = let _ = ord.TO.properties in ()
+
+let compare_eq_of_eq (a:Type0) (ord:erased (TO.total_order a)) (x y:a)
+  : Lemma (requires x == y) (ensures eq (x `ord.TO.compare` y) = true)
+  = let _ = ord.TO.properties in ()
+
+let flip_gt_lt (a:Type0) (ord:erased (TO.total_order a)) (x y:a)
+  : Lemma (requires gt_ord a ord x y = true) (ensures lt_ord a ord y x = true)
+  = reveal_ord a ord
+
+let flip_lt_gt (a:Type0) (ord:erased (TO.total_order a)) (x y:a)
+  : Lemma (requires lt_ord a ord x y = true) (ensures gt_ord a ord y x = true)
+  = reveal_ord a ord
+
+let lt_trans (a:Type0) (ord:erased (TO.total_order a)) (x y z:a)
+  : Lemma (requires lt_ord a ord x y /\ lt_ord a ord y z)
+          (ensures lt_ord a ord x z)
+  = reveal_ord a ord
+
+let gt_trans (a:Type0) (ord:erased (TO.total_order a)) (x y z:a)
+  : Lemma (requires gt_ord a ord x y /\ gt_ord a ord y z)
+          (ensures gt_ord a ord x z)
+  = reveal_ord a ord
+
+let compare_lt_trans (a:Type0) (ord:erased (TO.total_order a)) (x y z:a)
+  : Lemma (requires lt (ord.TO.compare x y) /\ lt (ord.TO.compare y z))
+          (ensures lt (ord.TO.compare x z))
+  = reveal_ord a ord
+
+#push-options "--fuel 2 --ifuel 1 --z3rlimit 10"
+let rec find_none_all_lt (a:Type0) (ord:erased (TO.total_order a)) (t:rbtree a) (key:a)
+  : Lemma
+      (requires all_lt a ord t key = true)
+      (ensures find_model a ord t key == None)
+      (decreases t)
+  =
+  reveal_ord a ord;
+  match t with
+  | Leaf -> ()
+  | Node _ l k r ->
+      find_none_all_lt a ord l key;
+      find_none_all_lt a ord r key
+
+let rec find_none_all_gt (a:Type0) (ord:erased (TO.total_order a)) (t:rbtree a) (key:a)
+  : Lemma
+      (requires all_gt a ord t key = true)
+      (ensures find_model a ord t key == None)
+      (decreases t)
+  =
+  reveal_ord a ord;
+  match t with
+  | Leaf -> ()
+  | Node _ l k r ->
+      find_none_all_gt a ord l key;
+      find_none_all_gt a ord r key
+
+let rec find_some_all_lt_poly (a:Type0) (ord:erased (TO.total_order a)) (t:rbtree a) (bound:a) (key:a)
+  : Lemma
+      (requires all_lt a ord t bound /\ Some? (find_model a ord t key))
+      (ensures lt_ord a ord key bound)
+      (decreases t)
+  =
+  reveal_ord a ord;
+  match t with
+  | Leaf -> ()
+  | Node _ l v r ->
+      let cmp = key `ord.TO.compare` v in
+      if lt cmp then find_some_all_lt_poly a ord l bound key
+      else if gt cmp then find_some_all_lt_poly a ord r bound key
+      else compare_eq_is_eq a ord key v
+
+let rec find_some_all_gt_poly (a:Type0) (ord:erased (TO.total_order a)) (t:rbtree a) (bound:a) (key:a)
+  : Lemma
+      (requires all_gt a ord t bound /\ Some? (find_model a ord t key))
+      (ensures gt_ord a ord key bound)
+      (decreases t)
+  =
+  reveal_ord a ord;
+  match t with
+  | Leaf -> ()
+  | Node _ l v r ->
+      let cmp = key `ord.TO.compare` v in
+      if lt cmp then find_some_all_gt_poly a ord l bound key
+      else if gt cmp then find_some_all_gt_poly a ord r bound key
+      else compare_eq_is_eq a ord key v
+#pop-options
+
+#push-options "--fuel 2 --ifuel 1 --z3rlimit 10"
+let rec all_lt_weaken_poly (a:Type0) (ord:erased (TO.total_order a)) (t:rbtree a) (b1 b2:a)
+  : Lemma (requires all_lt a ord t b1 /\ lt_ord a ord b1 b2) (ensures all_lt a ord t b2)
+          (decreases t)
+  = reveal_ord a ord;
+    match t with | Leaf -> () | Node _ l _ r ->
+      all_lt_weaken_poly a ord l b1 b2; all_lt_weaken_poly a ord r b1 b2
+
+let rec all_gt_weaken_poly (a:Type0) (ord:erased (TO.total_order a)) (t:rbtree a) (b1 b2:a)
+  : Lemma (requires all_gt a ord t b1 /\ gt_ord a ord b1 b2) (ensures all_gt a ord t b2)
+          (decreases t)
+  = reveal_ord a ord;
+    match t with | Leaf -> () | Node _ l _ r ->
+      all_gt_weaken_poly a ord l b1 b2; all_gt_weaken_poly a ord r b1 b2
+#pop-options
+
 let left_rotate (a:Type0) (t:rbtree a) : rbtree a =
   match t with
   | Node c a_ x (Node rc b y d) -> Node rc (Node c a_ x b) y d
@@ -71,6 +239,84 @@ let right_rotate (a:Type0) (t:rbtree a) : rbtree a =
   match t with
   | Node c (Node lc a_ x b) y d -> Node lc a_ x (Node c b y d)
   | _ -> t
+
+// ===== Rotation Lemmas =====
+
+#push-options "--fuel 3 --ifuel 2 --z3rlimit 15"
+let right_rotate_all_lt
+    (a:Type0) (ord:erased (TO.total_order a)) (c lc:color)
+    (p:rbtree a) (x:a) (q:rbtree a) (y:a) (r:rbtree a) (bound:a)
+  : Lemma (requires all_lt a ord (Node c (Node lc p x q) y r) bound)
+          (ensures all_lt a ord (right_rotate a (Node c (Node lc p x q) y r)) bound)
+  = ()
+
+let right_rotate_all_gt
+    (a:Type0) (ord:erased (TO.total_order a)) (c lc:color)
+    (p:rbtree a) (x:a) (q:rbtree a) (y:a) (r:rbtree a) (bound:a)
+  : Lemma (requires all_gt a ord (Node c (Node lc p x q) y r) bound)
+          (ensures all_gt a ord (right_rotate a (Node c (Node lc p x q) y r)) bound)
+  = ()
+
+let left_rotate_all_lt
+    (a:Type0) (ord:erased (TO.total_order a)) (c rc:color)
+    (p:rbtree a) (x:a) (q:rbtree a) (y:a) (r:rbtree a) (bound:a)
+  : Lemma (requires all_lt a ord (Node c p x (Node rc q y r)) bound)
+          (ensures all_lt a ord (left_rotate a (Node c p x (Node rc q y r))) bound)
+  = ()
+
+let left_rotate_all_gt
+    (a:Type0) (ord:erased (TO.total_order a)) (c rc:color)
+    (p:rbtree a) (x:a) (q:rbtree a) (y:a) (r:rbtree a) (bound:a)
+  : Lemma (requires all_gt a ord (Node c p x (Node rc q y r)) bound)
+          (ensures all_gt a ord (left_rotate a (Node c p x (Node rc q y r))) bound)
+  = ()
+#pop-options
+
+#push-options "--fuel 4 --ifuel 2 --z3rlimit 20"
+let right_rotate_is_bst
+    (a:Type0) (ord:erased (TO.total_order a)) (c lc:color)
+    (p:rbtree a) (x:a) (q:rbtree a) (y:a) (r:rbtree a)
+  : Lemma (requires is_bst a ord (Node c (Node lc p x q) y r))
+          (ensures is_bst a ord (right_rotate a (Node c (Node lc p x q) y r)))
+  = reveal_ord a ord;
+    flip_lt_gt a ord x y;
+    all_gt_weaken_poly a ord r y x
+
+let left_rotate_is_bst
+    (a:Type0) (ord:erased (TO.total_order a)) (c rc:color)
+    (p:rbtree a) (x:a) (q:rbtree a) (y:a) (r:rbtree a)
+  : Lemma (requires is_bst a ord (Node c p x (Node rc q y r)))
+          (ensures is_bst a ord (left_rotate a (Node c p x (Node rc q y r))))
+  = reveal_ord a ord;
+    flip_gt_lt a ord y x;
+    all_lt_weaken_poly a ord p x y
+#pop-options
+
+#push-options "--fuel 4 --ifuel 2 --z3rlimit 20"
+let right_rotate_find
+    (a:Type0) (ord:erased (TO.total_order a)) (c lc:color)
+    (p:rbtree a) (x:a) (q:rbtree a) (y:a) (r:rbtree a) (key:a)
+  : Lemma (requires is_bst a ord (Node c (Node lc p x q) y r))
+          (ensures find_model a ord (right_rotate a (Node c (Node lc p x q) y r)) key ==
+                   find_model a ord (Node c (Node lc p x q) y r) key)
+  = reveal_ord a ord;
+    let cx = key `ord.TO.compare` x in
+    let cy = key `ord.TO.compare` y in
+    if eq cx then compare_eq_is_eq a ord key x
+    else if eq cy then compare_eq_is_eq a ord key y
+
+let left_rotate_find
+    (a:Type0) (ord:erased (TO.total_order a)) (c rc:color)
+    (p:rbtree a) (x:a) (q:rbtree a) (y:a) (r:rbtree a) (key:a)
+  : Lemma (requires is_bst a ord (Node c p x (Node rc q y r)))
+          (ensures find_model a ord (left_rotate a (Node c p x (Node rc q y r))) key ==
+                   find_model a ord (Node c p x (Node rc q y r)) key)
+  = reveal_ord a ord;
+    let cx = key `ord.TO.compare` x in
+    let cy = key `ord.TO.compare` y in
+    if eq cx then compare_eq_is_eq a ord key x
+    else if eq cy then compare_eq_is_eq a ord key y
+#pop-options
 
 let clrs_fixup_left (a:Type0) (c:color) (l:rbtree a) (v:a) (r:rbtree a) : rbtree a =
   match c with
@@ -102,6 +348,248 @@ let clrs_fixup_right (a:Type0) (c:color) (l:rbtree a) (v:a) (r:rbtree a) : rbtre
           else left_rotate a (Node Red l v (set_color a Black r))
       | _ -> Node Black l v r
 
+// ===== clrs_fixup_left / clrs_fixup_right BST + all_lt/all_gt Lemmas =====
+
+#push-options "--fuel 4 --ifuel 2 --z3rlimit 20"
+let clrs_fixup_left_all_lt
+    (a:Type0) (ord:erased (TO.total_order a)) (c:color) (l:rbtree a) (v:a) (r:rbtree a) (bound:a)
+  : Lemma (requires all_lt a ord l bound /\ all_lt a ord r bound /\ lt_ord a ord v bound)
+          (ensures all_lt a ord (clrs_fixup_left a c l v r) bound)
+  = match c with
+    | Red -> ()
+    | Black ->
+      match l with
+      | Node Red (Node Red gll glx glr) lv lr_ ->
+          if is_red_node a r then ()
+          else begin
+            set_color_all_lt a ord Black l bound;
+            right_rotate_all_lt a ord Red Black (Node Red gll glx glr) lv lr_ v r bound
+          end
+      | Node Red gll_ glx_ (Node Red grl grx grr) ->
+          if is_red_node a r then ()
+          else begin
+            left_rotate_all_lt a ord Red Red gll_ glx_ grl grx grr bound;
+            set_color_all_lt a ord Black (left_rotate a l) bound;
+            right_rotate_all_lt a ord Red Black (Node Red gll_ glx_ grl) grx grr v r bound
+          end
+      | _ -> ()
+
+let clrs_fixup_left_all_gt
+    (a:Type0) (ord:erased (TO.total_order a)) (c:color) (l:rbtree a) (v:a) (r:rbtree a) (bound:a)
+  : Lemma (requires all_gt a ord l bound /\ all_gt a ord r bound /\ gt_ord a ord v bound)
+          (ensures all_gt a ord (clrs_fixup_left a c l v r) bound)
+  = match c with
+    | Red -> ()
+    | Black ->
+      match l with
+      | Node Red (Node Red gll glx glr) lv lr_ ->
+          if is_red_node a r then ()
+          else begin
+            set_color_all_gt a ord Black l bound;
+            right_rotate_all_gt a ord Red Black (Node Red gll glx glr) lv lr_ v r bound
+          end
+      | Node Red gll_ glx_ (Node Red grl grx grr) ->
+          if is_red_node a r then ()
+          else begin
+            left_rotate_all_gt a ord Red Red gll_ glx_ grl grx grr bound;
+            set_color_all_gt a ord Black (left_rotate a l) bound;
+            right_rotate_all_gt a ord Red Black (Node Red gll_ glx_ grl) grx grr v r bound
+          end
+      | _ -> ()
+
+let clrs_fixup_right_all_lt
+    (a:Type0) (ord:erased (TO.total_order a)) (c:color) (l:rbtree a) (v:a) (r:rbtree a) (bound:a)
+  : Lemma (requires all_lt a ord l bound /\ all_lt a ord r bound /\ lt_ord a ord v bound)
+          (ensures all_lt a ord (clrs_fixup_right a c l v r) bound)
+  = match c with
+    | Red -> ()
+    | Black ->
+      match r with
+      | Node Red (Node Red rll rlx rlr) rv rr ->
+          if is_red_node a l then ()
+          else begin
+            right_rotate_all_lt a ord Red Red rll rlx rlr rv rr bound;
+            set_color_all_lt a ord Black (right_rotate a r) bound;
+            left_rotate_all_lt a ord Red Black l v rll rlx (Node Red rlr rv rr) bound
+          end
+      | Node Red rll_ rlx_ (Node Red rrl rrx rrr) ->
+          if is_red_node a l then ()
+          else begin
+            set_color_all_lt a ord Black r bound;
+            left_rotate_all_lt a ord Red Black l v rll_ rlx_ (Node Red rrl rrx rrr) bound
+          end
+      | _ -> ()
+
+let clrs_fixup_right_all_gt
+    (a:Type0) (ord:erased (TO.total_order a)) (c:color) (l:rbtree a) (v:a) (r:rbtree a) (bound:a)
+  : Lemma (requires all_gt a ord l bound /\ all_gt a ord r bound /\ gt_ord a ord v bound)
+          (ensures all_gt a ord (clrs_fixup_right a c l v r) bound)
+  = match c with
+    | Red -> ()
+    | Black ->
+      match r with
+      | Node Red (Node Red rll rlx rlr) rv rr ->
+          if is_red_node a l then ()
+          else begin
+            right_rotate_all_gt a ord Red Red rll rlx rlr rv rr bound;
+            set_color_all_gt a ord Black (right_rotate a r) bound;
+            left_rotate_all_gt a ord Red Black l v rll rlx (Node Red rlr rv rr) bound
+          end
+      | Node Red rll_ rlx_ (Node Red rrl rrx rrr) ->
+          if is_red_node a l then ()
+          else begin
+            set_color_all_gt a ord Black r bound;
+            left_rotate_all_gt a ord Red Black l v rll_ rlx_ (Node Red rrl rrx rrr) bound
+          end
+      | _ -> ()
+#pop-options
+
+#push-options "--fuel 4 --ifuel 2 --z3rlimit 20"
+let clrs_fixup_left_is_bst
+    (a:Type0) (ord:erased (TO.total_order a)) (c:color) (l:rbtree a) (v:a) (r:rbtree a)
+  : Lemma (requires is_bst a ord l /\ is_bst a ord r /\ all_lt a ord l v /\ all_gt a ord r v)
+          (ensures is_bst a ord (clrs_fixup_left a c l v r))
+  = match c with
+    | Red -> ()
+    | Black ->
+      match l with
+      | Node Red (Node Red gll glx glr) lv lr_ ->
+          if is_red_node a r then begin
+            set_color_is_bst a ord Black l;
+            set_color_all_lt a ord Black l v;
+            set_color_is_bst a ord Black r;
+            set_color_all_gt a ord Black r v
+          end else begin
+            set_color_is_bst a ord Black l;
+            set_color_all_lt a ord Black l v;
+            right_rotate_is_bst a ord Red Black (Node Red gll glx glr) lv lr_ v r
+          end
+      | Node Red gll_ glx_ (Node Red grl grx grr) ->
+          if is_red_node a r then begin
+            set_color_is_bst a ord Black l;
+            set_color_all_lt a ord Black l v;
+            set_color_is_bst a ord Black r;
+            set_color_all_gt a ord Black r v
+          end else begin
+            left_rotate_is_bst a ord Red Red gll_ glx_ grl grx grr;
+            left_rotate_all_lt a ord Red Red gll_ glx_ grl grx grr v;
+            set_color_is_bst a ord Black (left_rotate a l);
+            set_color_all_lt a ord Black (left_rotate a l) v;
+            right_rotate_is_bst a ord Red Black (Node Red gll_ glx_ grl) grx grr v r
+          end
+      | _ -> ()
+
+let clrs_fixup_right_is_bst
+    (a:Type0) (ord:erased (TO.total_order a)) (c:color) (l:rbtree a) (v:a) (r:rbtree a)
+  : Lemma (requires is_bst a ord l /\ is_bst a ord r /\ all_lt a ord l v /\ all_gt a ord r v)
+          (ensures is_bst a ord (clrs_fixup_right a c l v r))
+  = match c with
+    | Red -> ()
+    | Black ->
+      match r with
+      | Node Red (Node Red rll rlx rlr) rv rr ->
+          if is_red_node a l then begin
+            set_color_is_bst a ord Black l;
+            set_color_all_lt a ord Black l v;
+            set_color_is_bst a ord Black r;
+            set_color_all_gt a ord Black r v
+          end else begin
+            right_rotate_is_bst a ord Red Red rll rlx rlr rv rr;
+            right_rotate_all_gt a ord Red Red rll rlx rlr rv rr v;
+            set_color_is_bst a ord Black (right_rotate a r);
+            set_color_all_gt a ord Black (right_rotate a r) v;
+            left_rotate_is_bst a ord Red Black l v rll rlx (Node Red rlr rv rr)
+          end
+      | Node Red rll_ rlx_ (Node Red rrl rrx rrr) ->
+          if is_red_node a l then begin
+            set_color_is_bst a ord Black l;
+            set_color_all_lt a ord Black l v;
+            set_color_is_bst a ord Black r;
+            set_color_all_gt a ord Black r v
+          end else begin
+            set_color_is_bst a ord Black r;
+            set_color_all_gt a ord Black r v;
+            left_rotate_is_bst a ord Red Black l v rll_ rlx_ (Node Red rrl rrx rrr)
+          end
+      | _ -> ()
+#pop-options
+
+#push-options "--fuel 4 --ifuel 2 --z3rlimit 20"
+let clrs_fixup_left_find
+    (a:Type0) (ord:erased (TO.total_order a)) (c:color) (l:rbtree a) (v:a) (r:rbtree a) (key:a)
+  : Lemma (requires is_bst a ord l /\ is_bst a ord r /\ all_lt a ord l v /\ all_gt a ord r v)
+          (ensures find_model a ord (clrs_fixup_left a c l v r) key ==
+                   find_model a ord (Node c l v r) key)
+  = reveal_ord a ord;
+    match c with
+    | Red -> ()
+    | Black ->
+      match l with
+      | Node Red (Node Red gll glx glr) lv lr_ ->
+          if is_red_node a r then begin
+            set_color_find a ord Black l key;
+            set_color_find a ord Black r key
+          end else begin
+            set_color_is_bst a ord Black l;
+            set_color_all_lt a ord Black l v;
+            right_rotate_is_bst a ord Red Black (Node Red gll glx glr) lv lr_ v r;
+            right_rotate_find a ord Red Black (Node Red gll glx glr) lv lr_ v r key;
+            set_color_find a ord Black l key
+          end
+      | Node Red gll_ glx_ (Node Red grl grx grr) ->
+          if is_red_node a r then begin
+            set_color_find a ord Black l key;
+            set_color_find a ord Black r key
+          end else begin
+            left_rotate_is_bst a ord Red Red gll_ glx_ grl grx grr;
+            left_rotate_all_lt a ord Red Red gll_ glx_ grl grx grr v;
+            left_rotate_find a ord Red Red gll_ glx_ grl grx grr key;
+            set_color_is_bst a ord Black (left_rotate a l);
+            set_color_all_lt a ord Black (left_rotate a l) v;
+            right_rotate_is_bst a ord Red Black (Node Red gll_ glx_ grl) grx grr v r;
+            right_rotate_find a ord Red Black (Node Red gll_ glx_ grl) grx grr v r key;
+            set_color_find a ord Black (left_rotate a l) key
+          end
+      | _ -> ()
+
+let clrs_fixup_right_find
+    (a:Type0) (ord:erased (TO.total_order a)) (c:color) (l:rbtree a) (v:a) (r:rbtree a) (key:a)
+  : Lemma (requires is_bst a ord l /\ is_bst a ord r /\ all_lt a ord l v /\ all_gt a ord r v)
+          (ensures find_model a ord (clrs_fixup_right a c l v r) key ==
+                   find_model a ord (Node c l v r) key)
+  = reveal_ord a ord;
+    match c with
+    | Red -> ()
+    | Black ->
+      match r with
+      | Node Red (Node Red rll rlx rlr) rv rr ->
+          if is_red_node a l then begin
+            set_color_find a ord Black l key;
+            set_color_find a ord Black r key
+          end else begin
+            right_rotate_is_bst a ord Red Red rll rlx rlr rv rr;
+            right_rotate_all_gt a ord Red Red rll rlx rlr rv rr v;
+            right_rotate_find a ord Red Red rll rlx rlr rv rr key;
+            set_color_is_bst a ord Black (right_rotate a r);
+            set_color_all_gt a ord Black (right_rotate a r) v;
+            left_rotate_is_bst a ord Red Black l v rll rlx (Node Red rlr rv rr);
+            left_rotate_find a ord Red Black l v rll rlx (Node Red rlr rv rr) key;
+            set_color_find a ord Black (right_rotate a r) key
+          end
+      | Node Red rll_ rlx_ (Node Red rrl rrx rrr) ->
+          if is_red_node a l then begin
+            set_color_find a ord Black l key;
+            set_color_find a ord Black r key
+          end else begin
+            set_color_is_bst a ord Black r;
+            set_color_all_gt a ord Black r v;
+            left_rotate_is_bst a ord Red Black l v rll_ rlx_ (Node Red rrl rrx rrr);
+            left_rotate_find a ord Red Black l v rll_ rlx_ (Node Red rrl rrx rrr) key;
+            set_color_find a ord Black r key
+          end
+      | _ -> ()
+#pop-options
+
 let rec clrs_ins_model (a:Type0) (ord:erased (TO.total_order a)) (t:rbtree a) (key:a)
   : GTot (rbtree a)
   =
@@ -117,6 +605,123 @@ let clrs_insert_model (a:Type0) (ord:erased (TO.total_order a)) (t:rbtree a) (ke
   : GTot (rbtree a)
   =
   make_black a (clrs_ins_model a ord t key)
+
+// ===== Insert BST + find Lemmas =====
+
+let make_black_find_poly (a:Type0) (ord:erased (TO.total_order a)) (t:rbtree a) (key:a)
+  : Lemma (ensures find_model a ord (make_black a t) key == find_model a ord t key)
+  = set_color_find a ord Black t key
+
+#push-options "--fuel 3 --ifuel 1 --z3rlimit 10"
+let rec clrs_ins_all_lt (a:Type0) (ord:erased (TO.total_order a)) (t:rbtree a) (k:a) (bound:a)
+  : Lemma (requires all_lt a ord t bound /\ lt_ord a ord k bound)
+          (ensures all_lt a ord (clrs_ins_model a ord t k) bound)
+          (decreases t)
+  = match t with | Leaf -> () | Node c l v r ->
+      reveal_ord a ord;
+      let cmp = k `ord.TO.compare` v in
+      if lt cmp then begin
+        clrs_ins_all_lt a ord l k bound;
+        clrs_fixup_left_all_lt a ord c (clrs_ins_model a ord l k) v r bound
+      end else if gt cmp then begin
+        clrs_ins_all_lt a ord r k bound;
+        clrs_fixup_right_all_lt a ord c l v (clrs_ins_model a ord r k) bound
+      end else ()
+
+let rec clrs_ins_all_gt (a:Type0) (ord:erased (TO.total_order a)) (t:rbtree a) (k:a) (bound:a)
+  : Lemma (requires all_gt a ord t bound /\ gt_ord a ord k bound)
+          (ensures all_gt a ord (clrs_ins_model a ord t k) bound)
+          (decreases t)
+  = match t with | Leaf -> () | Node c l v r ->
+      reveal_ord a ord;
+      let cmp = k `ord.TO.compare` v in
+      if lt cmp then begin
+        clrs_ins_all_gt a ord l k bound;
+        clrs_fixup_left_all_gt a ord c (clrs_ins_model a ord l k) v r bound
+      end else if gt cmp then begin
+        clrs_ins_all_gt a ord r k bound;
+        clrs_fixup_right_all_gt a ord c l v (clrs_ins_model a ord r k) bound
+      end else ()
+#pop-options
+
+#push-options "--fuel 4 --ifuel 2 --z3rlimit 20"
+let rec clrs_ins_preserves_bst (a:Type0) (ord:erased (TO.total_order a)) (t:rbtree a) (k:a)
+  : Lemma (requires is_bst a ord t) (ensures is_bst a ord (clrs_ins_model a ord t k))
+          (decreases t)
+  = match t with | Leaf -> () | Node c l v r ->
+      reveal_ord a ord;
+      let cmp = k `ord.TO.compare` v in
+      if lt cmp then begin
+        clrs_ins_preserves_bst a ord l k;
+        clrs_ins_all_lt a ord l k v;
+        clrs_fixup_left_is_bst a ord c (clrs_ins_model a ord l k) v r
+      end else if gt cmp then begin
+        clrs_ins_preserves_bst a ord r k;
+        clrs_ins_all_gt a ord r k v;
+        clrs_fixup_right_is_bst a ord c l v (clrs_ins_model a ord r k)
+      end else ()
+#pop-options
+
+let clrs_insert_model_valid (a:Type0) (ord:erased (TO.total_order a)) (t:rbtree a) (k:a)
+  : Lemma (requires valid a ord t) (ensures valid a ord (clrs_insert_model a ord t k))
+  = clrs_ins_preserves_bst a ord t k;
+    set_color_is_bst a ord Black (clrs_ins_model a ord t k)
+
+#push-options "--fuel 3 --ifuel 2 --z3rlimit 20"
+let rec find_ins_hit (a:Type0) (ord:erased (TO.total_order a)) (t:rbtree a) (key:a)
+  : Lemma (requires is_bst a ord t)
+          (ensures find_model a ord (clrs_ins_model a ord t key) key == Some key)
+          (decreases t)
+  = reveal_ord a ord;
+    match t with
+    | Leaf -> compare_eq_of_eq a ord key key
+    | Node c l k r ->
+      let cmp = key `ord.TO.compare` k in
+      if lt cmp then begin
+        find_ins_hit a ord l key;
+        clrs_ins_preserves_bst a ord l key;
+        clrs_ins_all_lt a ord l key k;
+        clrs_fixup_left_find a ord c (clrs_ins_model a ord l key) k r key
+      end else if gt cmp then begin
+        find_ins_hit a ord r key;
+        clrs_ins_preserves_bst a ord r key;
+        clrs_ins_all_gt a ord r key k;
+        clrs_fixup_right_find a ord c l k (clrs_ins_model a ord r key) key
+      end else compare_eq_is_eq a ord key k
+
+let rec find_ins_other (a:Type0) (ord:erased (TO.total_order a)) (t:rbtree a) (inserted key:a)
+  : Lemma (requires is_bst a ord t /\ SC.same_key a ord key inserted = false)
+          (ensures find_model a ord (clrs_ins_model a ord t inserted) key == find_model a ord t key)
+          (decreases t)
+  = reveal_ord a ord;
+    match t with
+    | Leaf -> ()
+    | Node c l k r ->
+      let cmpi = inserted `ord.TO.compare` k in
+      if lt cmpi then begin
+        find_ins_other a ord l inserted key;
+        clrs_ins_preserves_bst a ord l inserted;
+        clrs_ins_all_lt a ord l inserted k;
+        clrs_fixup_left_find a ord c (clrs_ins_model a ord l inserted) k r key
+      end else if gt cmpi then begin
+        find_ins_other a ord r inserted key;
+        clrs_ins_preserves_bst a ord r inserted;
+        clrs_ins_all_gt a ord r inserted k;
+        clrs_fixup_right_find a ord c l k (clrs_ins_model a ord r inserted) key
+      end else ()
+#pop-options
+
+let find_insert_hit (a:Type0) (ord:erased (TO.total_order a)) (m:rbtree a) (key:a)
+  : Lemma (requires valid a ord m)
+          (ensures find_model a ord (clrs_insert_model a ord m key) key == Some key)
+  = find_ins_hit a ord m key;
+    make_black_find_poly a ord (clrs_ins_model a ord m key) key
+
+let find_insert_other (a:Type0) (ord:erased (TO.total_order a)) (m:rbtree a) (inserted key:a)
+  : Lemma (requires valid a ord m /\ SC.same_key a ord key inserted = false)
+          (ensures find_model a ord (clrs_insert_model a ord m inserted) key == find_model a ord m key)
+  = find_ins_other a ord m inserted key;
+    make_black_find_poly a ord (clrs_ins_model a ord m inserted) key
 
 let rec minimum_model (a:Type0) (t:rbtree a) : option a =
   match t with
@@ -227,7 +832,753 @@ let clrs_delete_model (a:Type0) (ord:erased (TO.total_order a)) (t:rbtree a) (ke
   =
   make_black a (fst (clrs_del_model a ord t key))
 
-let valid (a:Type0) (_ord:erased (TO.total_order a)) (_t:rbtree a) : GTot prop = True
+let rec find_model_some_eq (a:Type0) (ord:erased (TO.total_order a)) (t:rbtree a) (key:a)
+  : Lemma
+      (requires Some? (find_model a ord t key))
+      (ensures Some?.v (find_model a ord t key) == key)
+      (decreases t)
+  =
+  reveal_ord a ord;
+  match t with
+  | Leaf -> ()
+  | Node _ l k r ->
+      let cmp = key `ord.TO.compare` k in
+      if lt cmp then find_model_some_eq a ord l key
+      else if gt cmp then find_model_some_eq a ord r key
+      else ()
+
+let find_empty (a:Type0) (ord:erased (TO.total_order a)) (key:a)
+  : Lemma (ensures find_model a ord (empty_model a) key == None)
+  = ()
+
+let rec minimum_nonempty (a:Type0) (t:rbtree a)
+  : Lemma (requires Node? t) (ensures Some? (minimum_model a t))
+          (decreases t)
+  = match t with
+    | Node _ Leaf _ _ -> ()
+    | Node _ l _ _ -> minimum_nonempty a l
+
+#push-options "--fuel 2 --ifuel 1 --z3rlimit 10"
+let rec minimum_in_all_lt (a:Type0) (ord:erased (TO.total_order a)) (t:rbtree a) (bound:a)
+  : Lemma (requires all_lt a ord t bound /\ Some? (minimum_model a t))
+          (ensures lt_ord a ord (Some?.v (minimum_model a t)) bound)
+          (decreases t)
+  = match t with
+    | Leaf -> ()
+    | Node _ Leaf _ _ -> ()
+    | Node _ l _ _ ->
+        minimum_nonempty a l;
+        minimum_in_all_lt a ord l bound
+
+let rec minimum_gt_bound (a:Type0) (ord:erased (TO.total_order a)) (t:rbtree a) (bound:a)
+  : Lemma (requires all_gt a ord t bound /\ Some? (minimum_model a t))
+          (ensures gt_ord a ord (Some?.v (minimum_model a t)) bound)
+          (decreases t)
+  = match t with
+    | Leaf -> ()
+    | Node _ Leaf _ _ -> ()
+    | Node _ l _ _ ->
+        minimum_nonempty a l;
+        minimum_gt_bound a ord l bound
+#pop-options
+
+let rec find_minimum_hit (a:Type0) (ord:erased (TO.total_order a)) (t:rbtree a)
+  : Lemma
+      (requires is_bst a ord t /\ Some? (minimum_model a t))
+      (ensures find_model a ord t (Some?.v (minimum_model a t)) ==
+               Some (Some?.v (minimum_model a t)))
+      (decreases t)
+  =
+  reveal_ord a ord;
+  match t with
+  | Leaf -> ()
+  | Node _ Leaf k r ->
+      compare_eq_of_eq a ord k k
+  | Node _ l k r ->
+      minimum_nonempty a l;
+      minimum_in_all_lt a ord l k;
+      find_minimum_hit a ord l
+
+let rec all_gt_of_lt_min (a:Type0) (ord:erased (TO.total_order a)) (t:rbtree a) (key:a)
+  : Lemma
+      (requires is_bst a ord t /\
+                Some? (minimum_model a t) /\
+                lt_ord a ord key (Some?.v (minimum_model a t)))
+      (ensures all_gt a ord t key)
+      (decreases t)
+  =
+  reveal_ord a ord;
+  match t with
+  | Leaf -> ()
+  | Node _ Leaf k r ->
+      flip_lt_gt a ord key k;
+      all_gt_weaken_poly a ord r k key
+  | Node _ l k r ->
+      minimum_nonempty a l;
+      minimum_in_all_lt a ord l k;
+      all_gt_of_lt_min a ord l key;
+      assert (lt_ord a ord key k = true);
+      flip_lt_gt a ord key k;
+      all_gt_weaken_poly a ord r k key
+
+let lt_min_of_lt_bound (a:Type0) (ord:erased (TO.total_order a)) (t:rbtree a) (bound key:a)
+  : Lemma
+      (requires all_gt a ord t bound /\ Some? (minimum_model a t) /\ lt_ord a ord key bound)
+      (ensures lt (ord.TO.compare key (Some?.v (minimum_model a t))))
+  =
+  minimum_gt_bound a ord t bound;
+  flip_gt_lt a ord (Some?.v (minimum_model a t)) bound;
+  compare_lt_trans a ord key bound (Some?.v (minimum_model a t))
+
+let find_left_of_successor_root
+    (a:Type0) (ord:erased (TO.total_order a)) (c:color)
+    (l r dr:rbtree a) (bound key successor:a)
+  : Lemma
+      (requires all_gt a ord r bound /\
+                Some? (minimum_model a r) /\
+                successor == Some?.v (minimum_model a r) /\
+                lt_ord a ord key bound)
+      (ensures find_model a ord (Node c l successor dr) key == find_model a ord l key)
+  =
+  lt_min_of_lt_bound a ord r bound key;
+  assert (ord.TO.compare key successor ==
+          ord.TO.compare key (Some?.v (minimum_model a r)));
+  assert (lt (ord.TO.compare key successor))
+
+#push-options "--fuel 4 --ifuel 2 --z3rlimit 20"
+let clrs_del_cases234_left_all_lt
+    (a:Type0) (ord:erased (TO.total_order a)) (c:color)
+    (x:rbtree a) (v:a) (w:rbtree a) (bound:a)
+  : Lemma (requires all_lt a ord x bound /\ all_lt a ord w bound /\ lt_ord a ord v bound)
+          (ensures all_lt a ord (fst (clrs_del_cases234_left a c x v w)) bound)
+  =
+  match w with
+  | Leaf -> ()
+  | Node wc wl wy wr ->
+      if Black? wc then
+        let wl_red = is_red_node a wl in
+        let wr_red = is_red_node a wr in
+        if not wl_red && not wr_red then ()
+        else if wr_red then set_color_all_lt a ord Black wr bound
+        else
+          match wl with
+          | Node Red _ _ _ -> ()
+          | Node Black _ _ _ -> ()
+          | Leaf -> ()
+
+let clrs_del_cases234_left_all_gt
+    (a:Type0) (ord:erased (TO.total_order a)) (c:color)
+    (x:rbtree a) (v:a) (w:rbtree a) (bound:a)
+  : Lemma (requires all_gt a ord x bound /\ all_gt a ord w bound /\ gt_ord a ord v bound)
+          (ensures all_gt a ord (fst (clrs_del_cases234_left a c x v w)) bound)
+  =
+  match w with
+  | Leaf -> ()
+  | Node wc wl wy wr ->
+      if Black? wc then
+        let wl_red = is_red_node a wl in
+        let wr_red = is_red_node a wr in
+        if not wl_red && not wr_red then ()
+        else if wr_red then set_color_all_gt a ord Black wr bound
+        else
+          match wl with
+          | Node Red _ _ _ -> ()
+          | Node Black _ _ _ -> ()
+          | Leaf -> ()
+
+let clrs_del_cases234_right_all_lt
+    (a:Type0) (ord:erased (TO.total_order a)) (c:color)
+    (w:rbtree a) (v:a) (x:rbtree a) (bound:a)
+  : Lemma (requires all_lt a ord w bound /\ all_lt a ord x bound /\ lt_ord a ord v bound)
+          (ensures all_lt a ord (fst (clrs_del_cases234_right a c w v x)) bound)
+  =
+  match w with
+  | Leaf -> ()
+  | Node wc wl wy wr ->
+      if Black? wc then
+        let wl_red = is_red_node a wl in
+        let wr_red = is_red_node a wr in
+        if not wl_red && not wr_red then ()
+        else if wl_red then set_color_all_lt a ord Black wl bound
+        else
+          match wr with
+          | Node Red _ _ _ -> ()
+          | Node Black _ _ _ -> ()
+          | Leaf -> ()
+
+let clrs_del_cases234_right_all_gt
+    (a:Type0) (ord:erased (TO.total_order a)) (c:color)
+    (w:rbtree a) (v:a) (x:rbtree a) (bound:a)
+  : Lemma (requires all_gt a ord w bound /\ all_gt a ord x bound /\ gt_ord a ord v bound)
+          (ensures all_gt a ord (fst (clrs_del_cases234_right a c w v x)) bound)
+  =
+  match w with
+  | Leaf -> ()
+  | Node wc wl wy wr ->
+      if Black? wc then
+        let wl_red = is_red_node a wl in
+        let wr_red = is_red_node a wr in
+        if not wl_red && not wr_red then ()
+        else if wl_red then set_color_all_gt a ord Black wl bound
+        else
+          match wr with
+          | Node Red _ _ _ -> ()
+          | Node Black _ _ _ -> ()
+          | Leaf -> ()
+#pop-options
+
+#push-options "--fuel 4 --ifuel 2 --z3rlimit 20"
+let clrs_del_cases234_left_is_bst
+    (a:Type0) (ord:erased (TO.total_order a)) (c:color)
+    (x:rbtree a) (v:a) (w:rbtree a)
+  : Lemma (requires is_bst a ord x /\ is_bst a ord w /\ all_lt a ord x v /\ all_gt a ord w v)
+          (ensures is_bst a ord (fst (clrs_del_cases234_left a c x v w)))
+  =
+  reveal_ord a ord;
+  match w with
+  | Leaf -> ()
+  | Node wc wl wy wr ->
+      if Black? wc then
+        let wl_red = is_red_node a wl in
+        let wr_red = is_red_node a wr in
+        if not wl_red && not wr_red then ()
+        else if wr_red then begin
+          flip_gt_lt a ord wy v;
+          all_lt_weaken_poly a ord x v wy;
+          set_color_is_bst a ord Black wr;
+          set_color_all_gt a ord Black wr wy
+        end else
+          match wl with
+          | Node Red wll wlv wlr ->
+              flip_gt_lt a ord wlv v;
+              all_lt_weaken_poly a ord x v wlv;
+              flip_lt_gt a ord wlv wy;
+              all_gt_weaken_poly a ord wr wy wlv
+          | Node Black wll wlv wlr ->
+              flip_gt_lt a ord wlv v;
+              all_lt_weaken_poly a ord x v wlv;
+              flip_lt_gt a ord wlv wy;
+              all_gt_weaken_poly a ord wr wy wlv
+          | Leaf -> ()
+
+let clrs_del_cases234_right_is_bst
+    (a:Type0) (ord:erased (TO.total_order a)) (c:color)
+    (w:rbtree a) (v:a) (x:rbtree a)
+  : Lemma (requires is_bst a ord w /\ is_bst a ord x /\ all_lt a ord w v /\ all_gt a ord x v)
+          (ensures is_bst a ord (fst (clrs_del_cases234_right a c w v x)))
+  =
+  reveal_ord a ord;
+  match w with
+  | Leaf -> ()
+  | Node wc wl wy wr ->
+      if Black? wc then
+        let wl_red = is_red_node a wl in
+        let wr_red = is_red_node a wr in
+        if not wl_red && not wr_red then ()
+        else if wl_red then begin
+          flip_lt_gt a ord wy v;
+          all_gt_weaken_poly a ord x v wy;
+          set_color_is_bst a ord Black wl;
+          set_color_all_lt a ord Black wl wy
+        end else
+          match wr with
+          | Node Red wrl wrv wrr ->
+              flip_lt_gt a ord wrv v;
+              all_gt_weaken_poly a ord x v wrv;
+              flip_gt_lt a ord wrv wy;
+              all_lt_weaken_poly a ord wl wy wrv
+          | Node Black wrl wrv wrr ->
+              flip_lt_gt a ord wrv v;
+              all_gt_weaken_poly a ord x v wrv;
+              flip_gt_lt a ord wrv wy;
+              all_lt_weaken_poly a ord wl wy wrv
+          | Leaf -> ()
+#pop-options
+
+#push-options "--fuel 4 --ifuel 2 --z3rlimit 20"
+let clrs_resolve_left_all_lt
+    (a:Type0) (ord:erased (TO.total_order a)) (c:color)
+    (x:rbtree a) (v:a) (w:rbtree a) (bound:a)
+  : Lemma (requires all_lt a ord x bound /\ all_lt a ord w bound /\ lt_ord a ord v bound)
+          (ensures all_lt a ord (fst (clrs_resolve_left a c x v w)) bound)
+  =
+  match w with
+  | Leaf -> ()
+  | Node wc wl wy wr ->
+      if Red? wc then
+        clrs_del_cases234_left_all_lt a ord Red x v wl bound
+      else
+        clrs_del_cases234_left_all_lt a ord c x v w bound
+
+let clrs_resolve_left_all_gt
+    (a:Type0) (ord:erased (TO.total_order a)) (c:color)
+    (x:rbtree a) (v:a) (w:rbtree a) (bound:a)
+  : Lemma (requires all_gt a ord x bound /\ all_gt a ord w bound /\ gt_ord a ord v bound)
+          (ensures all_gt a ord (fst (clrs_resolve_left a c x v w)) bound)
+  =
+  match w with
+  | Leaf -> ()
+  | Node wc wl wy wr ->
+      if Red? wc then
+        clrs_del_cases234_left_all_gt a ord Red x v wl bound
+      else
+        clrs_del_cases234_left_all_gt a ord c x v w bound
+
+let clrs_resolve_right_all_lt
+    (a:Type0) (ord:erased (TO.total_order a)) (c:color)
+    (w:rbtree a) (v:a) (x:rbtree a) (bound:a)
+  : Lemma (requires all_lt a ord w bound /\ all_lt a ord x bound /\ lt_ord a ord v bound)
+          (ensures all_lt a ord (fst (clrs_resolve_right a c w v x)) bound)
+  =
+  match w with
+  | Leaf -> ()
+  | Node wc wl wy wr ->
+      if Red? wc then
+        clrs_del_cases234_right_all_lt a ord Red wr v x bound
+      else
+        clrs_del_cases234_right_all_lt a ord c w v x bound
+
+let clrs_resolve_right_all_gt
+    (a:Type0) (ord:erased (TO.total_order a)) (c:color)
+    (w:rbtree a) (v:a) (x:rbtree a) (bound:a)
+  : Lemma (requires all_gt a ord w bound /\ all_gt a ord x bound /\ gt_ord a ord v bound)
+          (ensures all_gt a ord (fst (clrs_resolve_right a c w v x)) bound)
+  =
+  match w with
+  | Leaf -> ()
+  | Node wc wl wy wr ->
+      if Red? wc then
+        clrs_del_cases234_right_all_gt a ord Red wr v x bound
+      else
+        clrs_del_cases234_right_all_gt a ord c w v x bound
+#pop-options
+
+#push-options "--fuel 4 --ifuel 2 --z3rlimit 20"
+let clrs_resolve_left_is_bst
+    (a:Type0) (ord:erased (TO.total_order a)) (c:color)
+    (x:rbtree a) (v:a) (w:rbtree a)
+  : Lemma (requires is_bst a ord x /\ is_bst a ord w /\ all_lt a ord x v /\ all_gt a ord w v)
+          (ensures is_bst a ord (fst (clrs_resolve_left a c x v w)))
+  =
+  reveal_ord a ord;
+  match w with
+  | Leaf -> ()
+  | Node wc wl wy wr ->
+      if Red? wc then begin
+        flip_gt_lt a ord wy v;
+        all_lt_weaken_poly a ord x v wy;
+        clrs_del_cases234_left_is_bst a ord Red x v wl;
+        clrs_del_cases234_left_all_lt a ord Red x v wl wy
+      end else
+        clrs_del_cases234_left_is_bst a ord c x v w
+
+let clrs_resolve_right_is_bst
+    (a:Type0) (ord:erased (TO.total_order a)) (c:color)
+    (w:rbtree a) (v:a) (x:rbtree a)
+  : Lemma (requires is_bst a ord w /\ is_bst a ord x /\ all_lt a ord w v /\ all_gt a ord x v)
+          (ensures is_bst a ord (fst (clrs_resolve_right a c w v x)))
+  =
+  reveal_ord a ord;
+  match w with
+  | Leaf -> ()
+  | Node wc wl wy wr ->
+      if Red? wc then begin
+        flip_lt_gt a ord wy v;
+        all_gt_weaken_poly a ord x v wy;
+        clrs_del_cases234_right_is_bst a ord Red wr v x;
+        clrs_del_cases234_right_all_gt a ord Red wr v x wy
+      end else
+        clrs_del_cases234_right_is_bst a ord c w v x
+#pop-options
+
+#push-options "--fuel 3 --ifuel 2 --z3rlimit 20"
+let rec clrs_del_all_lt (a:Type0) (ord:erased (TO.total_order a)) (t:rbtree a) (key bound:a)
+  : Lemma (requires is_bst a ord t /\ all_lt a ord t bound)
+          (ensures all_lt a ord (fst (clrs_del_model a ord t key)) bound)
+          (decreases t)
+  =
+  match t with
+  | Leaf -> ()
+  | Node c l k r ->
+      let cmp = key `ord.TO.compare` k in
+      if lt cmp then begin
+        clrs_del_all_lt a ord l key bound;
+        if snd (clrs_del_model a ord l key) then
+          clrs_resolve_left_all_lt a ord c (fst (clrs_del_model a ord l key)) k r bound
+      end else if gt cmp then begin
+        clrs_del_all_lt a ord r key bound;
+        if snd (clrs_del_model a ord r key) then
+          clrs_resolve_right_all_lt a ord c l k (fst (clrs_del_model a ord r key)) bound
+      end else
+        match l, r with
+        | Leaf, _ -> ()
+        | _, Leaf -> ()
+        | _, _ ->
+            match minimum_model a r with
+            | None -> ()
+            | Some successor ->
+                minimum_in_all_lt a ord r bound;
+                clrs_del_all_lt a ord r successor bound;
+                if snd (clrs_del_model a ord r successor) then
+                  clrs_resolve_right_all_lt a ord c l successor (fst (clrs_del_model a ord r successor)) bound
+
+let rec clrs_del_all_gt (a:Type0) (ord:erased (TO.total_order a)) (t:rbtree a) (key bound:a)
+  : Lemma (requires is_bst a ord t /\ all_gt a ord t bound)
+          (ensures all_gt a ord (fst (clrs_del_model a ord t key)) bound)
+          (decreases t)
+  =
+  match t with
+  | Leaf -> ()
+  | Node c l k r ->
+      let cmp = key `ord.TO.compare` k in
+      if lt cmp then begin
+        clrs_del_all_gt a ord l key bound;
+        if snd (clrs_del_model a ord l key) then
+          clrs_resolve_left_all_gt a ord c (fst (clrs_del_model a ord l key)) k r bound
+      end else if gt cmp then begin
+        clrs_del_all_gt a ord r key bound;
+        if snd (clrs_del_model a ord r key) then
+          clrs_resolve_right_all_gt a ord c l k (fst (clrs_del_model a ord r key)) bound
+      end else
+        match l, r with
+        | Leaf, _ -> ()
+        | _, Leaf -> ()
+        | _, _ ->
+            match minimum_model a r with
+            | None -> ()
+            | Some successor ->
+                minimum_gt_bound a ord r bound;
+                clrs_del_all_gt a ord r successor bound;
+                if snd (clrs_del_model a ord r successor) then
+                  clrs_resolve_right_all_gt a ord c l successor (fst (clrs_del_model a ord r successor)) bound
+#pop-options
+
+#push-options "--fuel 3 --ifuel 2 --z3rlimit 20"
+let rec clrs_del_all_gt_min (a:Type0) (ord:erased (TO.total_order a)) (t:rbtree a)
+  : Lemma (requires is_bst a ord t /\ Some? (minimum_model a t))
+          (ensures (let m = Some?.v (minimum_model a t) in
+                    all_gt a ord (fst (clrs_del_model a ord t m)) m))
+          (decreases t)
+  =
+  reveal_ord a ord;
+  match t with
+  | Leaf -> ()
+  | Node c Leaf k r -> ()
+  | Node c l k r ->
+      minimum_nonempty a l;
+      let m = Some?.v (minimum_model a l) in
+      minimum_in_all_lt a ord l k;
+      flip_lt_gt a ord m k;
+      clrs_del_all_gt_min a ord l;
+      all_gt_weaken_poly a ord r k m;
+      if snd (clrs_del_model a ord l m) then
+        clrs_resolve_left_all_gt a ord c (fst (clrs_del_model a ord l m)) k r m
+#pop-options
+
+#push-options "--fuel 3 --ifuel 2 --z3rlimit 20"
+let rec clrs_del_preserves_bst (a:Type0) (ord:erased (TO.total_order a)) (t:rbtree a) (key:a)
+  : Lemma (requires is_bst a ord t)
+          (ensures is_bst a ord (fst (clrs_del_model a ord t key)))
+          (decreases t)
+  =
+  reveal_ord a ord;
+  match t with
+  | Leaf -> ()
+  | Node c l k r ->
+      let cmp = key `ord.TO.compare` k in
+      if lt cmp then begin
+        clrs_del_preserves_bst a ord l key;
+        clrs_del_all_lt a ord l key k;
+        if snd (clrs_del_model a ord l key) then
+          clrs_resolve_left_is_bst a ord c (fst (clrs_del_model a ord l key)) k r
+      end else if gt cmp then begin
+        clrs_del_preserves_bst a ord r key;
+        clrs_del_all_gt a ord r key k;
+        if snd (clrs_del_model a ord r key) then
+          clrs_resolve_right_is_bst a ord c l k (fst (clrs_del_model a ord r key))
+      end else
+        match l, r with
+        | Leaf, _ -> ()
+        | _, Leaf -> ()
+        | _, _ ->
+            match minimum_model a r with
+            | None -> ()
+            | Some successor ->
+                clrs_del_preserves_bst a ord r successor;
+                minimum_gt_bound a ord r k;
+                flip_gt_lt a ord successor k;
+                all_lt_weaken_poly a ord l k successor;
+                clrs_del_all_gt_min a ord r;
+                if snd (clrs_del_model a ord r successor) then
+                  clrs_resolve_right_is_bst a ord c l successor (fst (clrs_del_model a ord r successor))
+#pop-options
+
+let clrs_delete_model_valid (a:Type0) (ord:erased (TO.total_order a)) (t:rbtree a) (key:a)
+  : Lemma (requires valid a ord t) (ensures valid a ord (clrs_delete_model a ord t key))
+  = clrs_del_preserves_bst a ord t key;
+    set_color_is_bst a ord Black (fst (clrs_del_model a ord t key))
+
+#push-options "--fuel 5 --ifuel 3 --z3rlimit 20"
+let clrs_del_cases234_left_find
+    (a:Type0) (ord:erased (TO.total_order a)) (c:color)
+    (x:rbtree a) (v:a) (w:rbtree a) (key:a)
+  : Lemma (requires is_bst a ord x /\ is_bst a ord w /\ all_lt a ord x v /\ all_gt a ord w v)
+          (ensures find_model a ord (fst (clrs_del_cases234_left a c x v w)) key ==
+                   find_model a ord (Node c x v w) key)
+  =
+  reveal_ord a ord;
+  match w with
+  | Leaf -> ()
+  | Node wc wl wy wr ->
+      let cv = key `ord.TO.compare` v in
+      let cy = key `ord.TO.compare` wy in
+      if Black? wc then
+        let wl_red = is_red_node a wl in
+        let wr_red = is_red_node a wr in
+        if not wl_red && not wr_red then ()
+        else if wr_red then begin
+          set_color_find a ord Black wr key;
+          if eq cv then compare_eq_is_eq a ord key v;
+          if eq cy then compare_eq_is_eq a ord key wy
+        end else
+          match wl with
+          | Node Red wll wlv wlr ->
+              let clv = key `ord.TO.compare` wlv in
+              if eq cv then compare_eq_is_eq a ord key v;
+              if eq clv then compare_eq_is_eq a ord key wlv;
+              if eq cy then compare_eq_is_eq a ord key wy
+          | Node Black wll wlv wlr ->
+              let clv = key `ord.TO.compare` wlv in
+              if eq cv then compare_eq_is_eq a ord key v;
+              if eq clv then compare_eq_is_eq a ord key wlv;
+              if eq cy then compare_eq_is_eq a ord key wy
+          | Leaf -> ()
+
+let clrs_del_cases234_right_find
+    (a:Type0) (ord:erased (TO.total_order a)) (c:color)
+    (w:rbtree a) (v:a) (x:rbtree a) (key:a)
+  : Lemma (requires is_bst a ord w /\ is_bst a ord x /\ all_lt a ord w v /\ all_gt a ord x v)
+          (ensures find_model a ord (fst (clrs_del_cases234_right a c w v x)) key ==
+                   find_model a ord (Node c w v x) key)
+  =
+  reveal_ord a ord;
+  match w with
+  | Leaf -> ()
+  | Node wc wl wy wr ->
+      let cv = key `ord.TO.compare` v in
+      let cy = key `ord.TO.compare` wy in
+      if Black? wc then
+        let wl_red = is_red_node a wl in
+        let wr_red = is_red_node a wr in
+        if not wl_red && not wr_red then ()
+        else if wl_red then begin
+          set_color_find a ord Black wl key;
+          if eq cv then compare_eq_is_eq a ord key v;
+          if eq cy then compare_eq_is_eq a ord key wy
+        end else
+          match wr with
+          | Node Red wrl wrv wrr ->
+              let crv = key `ord.TO.compare` wrv in
+              if eq cv then compare_eq_is_eq a ord key v;
+              if eq cy then compare_eq_is_eq a ord key wy;
+              if eq crv then compare_eq_is_eq a ord key wrv
+          | Node Black wrl wrv wrr ->
+              let crv = key `ord.TO.compare` wrv in
+              if eq cv then compare_eq_is_eq a ord key v;
+              if eq cy then compare_eq_is_eq a ord key wy;
+              if eq crv then compare_eq_is_eq a ord key wrv
+          | Leaf -> ()
+
+let clrs_resolve_left_find
+    (a:Type0) (ord:erased (TO.total_order a)) (c:color)
+    (x:rbtree a) (v:a) (w:rbtree a) (key:a)
+  : Lemma (requires is_bst a ord x /\ is_bst a ord w /\ all_lt a ord x v /\ all_gt a ord w v)
+          (ensures find_model a ord (fst (clrs_resolve_left a c x v w)) key ==
+                   find_model a ord (Node c x v w) key)
+  =
+  reveal_ord a ord;
+  match w with
+  | Leaf -> ()
+  | Node wc wl wy wr ->
+      let cv = key `ord.TO.compare` v in
+      let cy = key `ord.TO.compare` wy in
+      if Red? wc then begin
+        clrs_del_cases234_left_find a ord Red x v wl key;
+        if eq cv then compare_eq_is_eq a ord key v;
+        if eq cy then compare_eq_is_eq a ord key wy
+      end else
+        clrs_del_cases234_left_find a ord c x v w key
+
+let clrs_resolve_right_find
+    (a:Type0) (ord:erased (TO.total_order a)) (c:color)
+    (w:rbtree a) (v:a) (x:rbtree a) (key:a)
+  : Lemma (requires is_bst a ord w /\ is_bst a ord x /\ all_lt a ord w v /\ all_gt a ord x v)
+          (ensures find_model a ord (fst (clrs_resolve_right a c w v x)) key ==
+                   find_model a ord (Node c w v x) key)
+  =
+  reveal_ord a ord;
+  match w with
+  | Leaf -> ()
+  | Node wc wl wy wr ->
+      let cv = key `ord.TO.compare` v in
+      let cy = key `ord.TO.compare` wy in
+      if Red? wc then begin
+        clrs_del_cases234_right_find a ord Red wr v x key;
+        if eq cv then compare_eq_is_eq a ord key v;
+        if eq cy then compare_eq_is_eq a ord key wy
+      end else
+        clrs_del_cases234_right_find a ord c w v x key
+#pop-options
+
+#push-options "--fuel 3 --ifuel 2 --z3rlimit 20"
+let rec find_clrs_del_hit (a:Type0) (ord:erased (TO.total_order a)) (t:rbtree a) (key:a)
+  : Lemma (requires is_bst a ord t)
+          (ensures find_model a ord (fst (clrs_del_model a ord t key)) key == None)
+          (decreases t)
+  =
+  reveal_ord a ord;
+  match t with
+  | Leaf -> ()
+  | Node c l k r ->
+      let cmp = key `ord.TO.compare` k in
+      if lt cmp then begin
+        find_clrs_del_hit a ord l key;
+        clrs_del_preserves_bst a ord l key;
+        clrs_del_all_lt a ord l key k;
+        if snd (clrs_del_model a ord l key) then
+          clrs_resolve_left_find a ord c (fst (clrs_del_model a ord l key)) k r key
+      end else if gt cmp then begin
+        find_clrs_del_hit a ord r key;
+        clrs_del_preserves_bst a ord r key;
+        clrs_del_all_gt a ord r key k;
+        if snd (clrs_del_model a ord r key) then
+          clrs_resolve_right_find a ord c l k (fst (clrs_del_model a ord r key)) key
+      end else begin
+        compare_eq_is_eq a ord key k;
+        match l, r with
+        | Leaf, _ ->
+            set_color_find a ord Black r key;
+            find_none_all_gt a ord r key
+        | _, Leaf ->
+            set_color_find a ord Black l key;
+            find_none_all_lt a ord l key
+        | _, _ ->
+            minimum_nonempty a r;
+            match minimum_model a r with
+            | None -> ()
+            | Some successor ->
+                minimum_gt_bound a ord r key;
+                flip_gt_lt a ord successor key;
+                all_lt_weaken_poly a ord l key successor;
+                find_none_all_lt a ord l key;
+                clrs_del_preserves_bst a ord r successor;
+                clrs_del_all_gt_min a ord r;
+                if snd (clrs_del_model a ord r successor) then
+                  clrs_resolve_right_find a ord c l successor (fst (clrs_del_model a ord r successor)) key
+      end
+
+let rec find_clrs_del_other (a:Type0) (ord:erased (TO.total_order a)) (t:rbtree a) (deleted key:a)
+  : Lemma (requires is_bst a ord t /\ SC.same_key a ord key deleted = false)
+          (ensures find_model a ord (fst (clrs_del_model a ord t deleted)) key ==
+                   find_model a ord t key)
+          (decreases t)
+  =
+  reveal_ord a ord;
+  match t with
+  | Leaf -> ()
+  | Node c l k r ->
+      let cmpd = deleted `ord.TO.compare` k in
+      let cmpk = key `ord.TO.compare` k in
+      if lt cmpd then begin
+        find_clrs_del_other a ord l deleted key;
+        clrs_del_preserves_bst a ord l deleted;
+        clrs_del_all_lt a ord l deleted k;
+        if snd (clrs_del_model a ord l deleted) then
+          clrs_resolve_left_find a ord c (fst (clrs_del_model a ord l deleted)) k r key
+      end else if gt cmpd then begin
+        find_clrs_del_other a ord r deleted key;
+        clrs_del_preserves_bst a ord r deleted;
+        clrs_del_all_gt a ord r deleted k;
+        if snd (clrs_del_model a ord r deleted) then
+          clrs_resolve_right_find a ord c l k (fst (clrs_del_model a ord r deleted)) key
+      end else begin
+        compare_eq_is_eq a ord deleted k;
+        if lt cmpk then begin
+          match l, r with
+          | Leaf, _ ->
+              flip_lt_gt a ord key k;
+              all_gt_weaken_poly a ord r k key;
+              find_none_all_gt a ord r key;
+              set_color_find a ord Black r key
+          | _, Leaf -> ()
+          | _, _ ->
+              minimum_nonempty a r;
+              match minimum_model a r with
+              | None -> ()
+              | Some successor ->
+                  assert (successor == Some?.v (minimum_model a r));
+                  minimum_gt_bound a ord r k;
+                  flip_gt_lt a ord successor k;
+                  all_lt_weaken_poly a ord l k successor;
+                  clrs_del_preserves_bst a ord r successor;
+                  clrs_del_all_gt_min a ord r;
+                  find_left_of_successor_root a ord c l r (fst (clrs_del_model a ord r successor)) k key successor;
+                  if snd (clrs_del_model a ord r successor) then
+                    clrs_resolve_right_find a ord c l successor (fst (clrs_del_model a ord r successor)) key
+        end else if gt cmpk then begin
+          match l, r with
+          | Leaf, _ ->
+              set_color_find a ord Black r key
+          | _, Leaf ->
+              flip_gt_lt a ord key k;
+              all_lt_weaken_poly a ord l k key;
+              find_none_all_lt a ord l key;
+              set_color_find a ord Black l key
+          | _, _ ->
+              minimum_nonempty a r;
+              match minimum_model a r with
+              | None -> ()
+              | Some successor ->
+                  assert (successor == Some?.v (minimum_model a r));
+                  let cs = key `ord.TO.compare` successor in
+                  if lt cs then begin
+                    flip_gt_lt a ord key k;
+                    all_lt_weaken_poly a ord l k key;
+                    find_none_all_lt a ord l key;
+                    all_gt_of_lt_min a ord r key;
+                    find_none_all_gt a ord r key
+                  end else if gt cs then begin
+                    minimum_gt_bound a ord r k;
+                    flip_gt_lt a ord successor k;
+                    all_lt_weaken_poly a ord l k successor;
+                    find_clrs_del_other a ord r successor key;
+                    clrs_del_preserves_bst a ord r successor;
+                    clrs_del_all_gt_min a ord r;
+                    if snd (clrs_del_model a ord r successor) then
+                      clrs_resolve_right_find a ord c l successor (fst (clrs_del_model a ord r successor)) key
+                  end else begin
+                    compare_eq_is_eq a ord key successor;
+                    find_minimum_hit a ord r
+                  end
+        end else begin
+          compare_eq_is_eq a ord key k;
+          compare_eq_of_eq a ord key deleted;
+          assert (SC.same_key a ord key deleted = true)
+        end
+      end
+#pop-options
+
+let find_delete_hit (a:Type0) (ord:erased (TO.total_order a)) (m:rbtree a) (key:a)
+  : Lemma (requires valid a ord m)
+          (ensures find_model a ord (clrs_delete_model a ord m key) key == None)
+  = find_clrs_del_hit a ord m key;
+    make_black_find_poly a ord (fst (clrs_del_model a ord m key)) key
+
+let find_delete_other (a:Type0) (ord:erased (TO.total_order a)) (m:rbtree a) (deleted key:a)
+  : Lemma (requires valid a ord m /\ SC.same_key a ord key deleted = false)
+          (ensures find_model a ord (clrs_delete_model a ord m deleted) key == find_model a ord m key)
+  = find_clrs_del_other a ord m deleted key;
+    make_black_find_poly a ord (fst (clrs_del_model a ord m deleted)) key
 
 let rec search_ticks (a:Type0) (ord:erased (TO.total_order a)) (t:rbtree a) (key:a)
   : GTot nat
@@ -419,6 +1770,48 @@ ghost fn rbtree_case_some (a:Type0) (x:rb_ptr a) (bp:rb_node_ptr a)
   rewrite each x as (Some bp);
   cases_of_rbtree a (Some bp) ft parent;
   unfold (rbtree_cases a)
+}
+
+fn create (a:Type0)
+  (#ord:erased (TO.total_order a))
+  requires emp
+  returns tree:rb_ptr a
+  ensures owns a tree (empty_model a) ** pure (valid a ord (empty_model a))
+{
+  let tree : rb_ptr a = None #(rb_node_ptr a);
+  intro_leaf a tree (None #(rb_node_ptr a));
+  fold (owns a tree (empty_model a));
+  tree
+}
+
+fn rec free_rbtree (a:Type0) (tree:rb_ptr a)
+  requires rbtree_subtree a tree 'ft 'parent
+  ensures emp
+  decreases 'ft
+{
+  match tree {
+    None -> {
+      cases_of_rbtree a (None #(rb_node_ptr a)) 'ft 'parent;
+      unfold (rbtree_cases a)
+    }
+    Some bp -> {
+      rbtree_case_some a (Some bp) bp;
+      let node = !bp;
+      free_rbtree a node.left;
+      free_rbtree a node.right;
+      Box.free bp
+    }
+  }
+}
+
+fn dispose (a:Type0)
+  (tree:rb_ptr a)
+  (#m:erased (rbtree a))
+  requires owns a tree m
+  ensures emp
+{
+  unfold (owns a tree m);
+  free_rbtree a tree
 }
 
 ghost fn rbtree_not_leaf (a:Type0) (x:rb_ptr a) (#ft:rbtree a) (#parent:rb_ptr a)
@@ -1309,6 +2702,7 @@ fn insert (a:Type0)
   let tree' = clrs_insert_ptr a tree key (None #(rb_node_ptr a)) ctr #ord iord;
   with ticks. assert (MR.pts_to ctr #1.0R ticks);
   clrs_ins_ticks_bounded a ord m key;
+  clrs_insert_model_valid a ord m key;
   fold (owns a tree' (clrs_insert_model a ord m key));
   tree'
 }
@@ -1333,6 +2727,7 @@ fn delete (a:Type0)
   let tree' = clrs_delete_ptr a tree key (None #(rb_node_ptr a)) ctr #ord iord;
   with ticks. assert (MR.pts_to ctr #1.0R ticks);
   clrs_del_ticks_bounded a ord m key;
+  clrs_delete_model_valid a ord m key;
   fold (owns a tree' (clrs_delete_model a ord m key));
   tree'
 }
@@ -1343,6 +2738,7 @@ instance clrs_parent_pointer_search_structure_instance :
     rbtree
     owns
     valid
+    empty_model
     find_model
     clrs_insert_model
     clrs_delete_model
@@ -1352,7 +2748,25 @@ instance clrs_parent_pointer_search_structure_instance :
     insert_bound
     delete_bound
 = {
+  create = create;
+  dispose = dispose;
   search = search;
   insert = insert;
   delete = delete;
+}
+
+instance clrs_parent_pointer_search_model_laws_instance :
+  SC.search_model_laws
+    rbtree
+    valid
+    empty_model
+    find_model
+    clrs_insert_model
+    clrs_delete_model
+= {
+  find_empty = find_empty;
+  find_insert_hit = find_insert_hit;
+  find_insert_other = find_insert_other;
+  find_delete_hit = find_delete_hit;
+  find_delete_other = find_delete_other;
 }
